verification/specs_general.v
@@ -63,7 +63,7 @@ Proof.
 Qed.
 
 (** Custom notation with a list for PRE to make the specification better readable. *)
-Notation "'WITH'  x1 : t1 , x2 : t2 , x3 : t3 , x4 : t4 , x5 : t5 , x6 : t6 , x7 : t7 , x8 : t8 , x9 : t9 'PRE'  [[ xs ]] P 'POST' [ tz ] Q" :=
+Notation "'WITH'  x1 : t1 , x2 : t2 , x3 : t3 , x4 : t4 , x5 : t5 , x6 : t6 , x7 : t7 , x8 : t8 , x9 : t9 'PRE''  xs P 'POST' [ tz ] Q" :=
      (NDmk_funspec (xs, tz) cc_default (t1*t2*t3*t4*t5*t6*t7*t8*t9)
            (fun x => match x with (x1,x2,x3,x4,x5,x6,x7,x8,x9) => P%assert end)
            (fun x => match x with (x1,x2,x3,x4,x5,x6,x7,x8,x9) => Q%assert end))
@@ -84,7 +84,7 @@ Definition fn_desc_to_funspec_aux
   WITH gv : globals, g : graph, roots : GCGraph.roots_t, sh : share,
        xs : args c, ps : list rep_type, ti : val,
        outlier : GCGraph.outlier_t, t_info : GCGraph.thread_info
-   PRE [[ cons thread_info (repeat int_or_ptr_type arity) ]]
+   PRE' (cons thread_info (repeat int_or_ptr_type arity))
        PROP (writable_share sh ;
               prim_in_graphs g outlier c xs ps)
        (PARAMSx (ti :: map (rep_type_val g) ps)
@@ -113,7 +113,7 @@ Definition alloc_make_nat_S : funspec :=
   WITH gv : globals, g : graph, p : rep_type,
        x: nat, roots : roots_t, sh : share,
        ti : val, outlier : outlier_t, f_info : fun_info, t_info : GCGraph.thread_info
-  PRE  [[ [thread_info ; tulong] ]]
+  PRE'  [thread_info ; tulong]
      PROP (is_in_graph g x p ;
            writable_share sh)
      PARAMS (ti ; rep_type_val g p)
@@ -133,7 +133,7 @@ Definition alloc_make_spec_general
     WITH gv : globals, g : graph, ps : list rep_type,
          xs : args (ctor_reified c), roots : roots_t, sh : share,
          ti : val, outlier : outlier_t, t_info : GCGraph.thread_info
-    PRE  [[ thread_info :: repeat int_or_ptr_type n ]]
+    PRE'  (thread_info :: repeat int_or_ptr_type n)
        PROP (n = get_size (ctor_reified c) xs ;
              ctor_in_graphs g outlier _ xs ps ;
              (Z.of_nat n) < headroom t_info ;
